move the len methods to vec/slice_basic

theories/typing/lib/slice/slice_basic.v
@@ -5,7 +5,7 @@ Set Default Proof Using "Type".
 
 Implicit Type 𝔄 𝔅: syn_type.
 
-Section uniq_slice_basic.
+Section slice_basic.
   Context `{!typeG Σ}.
 
   Global Instance uniq_slice_type_contractive {𝔄} κ :
@@ -80,7 +80,41 @@ Section uniq_slice_basic.
     lctx_lft_eq E L κ' κ → eqtype E L ty ty' id id →
     eqtype E L (uniq_slice κ ty) (uniq_slice κ' ty') id id.
   Proof. move=> [??][??]. split; (apply uniq_slice_subtype; by [|split]). Qed.
-End uniq_slice_basic.
+
+  Definition slice_len: val :=
+    fn: ["bv"] :=
+      let: "v" := !"bv" in delete [ #1; "bv"];;
+      letalloc: "r" <- !("v" +ₗ #1) in
+      return: ["r"].
+
+  Lemma uniq_slice_len_type {𝔄} (ty: type 𝔄) :
+    typed_val slice_len (fn<(α, β)>(∅; &shr{β} (uniq_slice α ty)) → int)
+      (λ post '-[v], post (length v)).
+  Proof.
+    eapply type_fn; [apply _|]. move=>/= [α β]??[b[]]. simpl_subst.
+
+    iIntros (?[?[]]?) "LFT _ _ _ E Na L C /=[bv _] #Obs".
+    rewrite tctx_hasty_val. iDestruct "bv" as ([|d]) "[⧖ box]"=>//.
+    case b as [[]|]=>//=. rewrite split_mt_ptr.
+    case d as [|d]; first by iDestruct "box" as "[>[] _]".
+    iDestruct "box" as "[(%& >↦bv  & slice) †bv]". wp_read. wp_let.
+    rewrite -heap_mapsto_vec_singleton freeable_sz_full.
+    wp_apply (wp_delete with "[$↦bv $†bv]"); [done|]. iIntros "_". wp_seq.
+    case d as [|]=>//. iDestruct "slice" as (???? [Hsl ?]) "[Bor _]".
+    iMod (lctx_lft_alive_tok β with "E L") as (?) "(β & L & ToL)"; [solve_typing..|].
+    iMod (frac_bor_acc with "LFT Bor β") as (?) "[(↦₀ & ↦₁ & ↦₂) Toα]"; [done|].
+    wp_apply wp_new; [done..|]. iIntros (?) "[†r ↦r]". wp_let. wp_op. wp_read.
+    rewrite heap_mapsto_vec_singleton. wp_write. do 2 wp_seq.
+    iMod ("Toα" with "[$↦₀ $↦₁ $↦₂]") as "β". iMod ("ToL" with "β L") as "L".
+    rewrite cctx_interp_singleton. iApply ("C" $! [# #_] -[_] with "Na L [-] []").
+    - rewrite/= right_id (tctx_hasty_val #_) -freeable_sz_full. iExists _.
+      iFrame "⧖ †r". iNext. iExists [_]. rewrite heap_mapsto_vec_singleton.
+      iFrame "↦r". by iExists _.
+    - iApply proph_obs_eq; [|done]=>/= π. f_equal.
+      rewrite -(map_length fst). move: (equal_f Hsl π) => /= ->.
+      by rewrite -vec_to_list_apply vec_to_list_length.
+  Qed.
+End slice_basic.
 
 Global Hint Resolve uniq_slice_resolve uniq_slice_real
   uniq_slice_subtype uniq_slice_eqtype : lrust_typing.
